examples/unit-tests/testset.fst
@@ -1,4 +1,4 @@
-(* Expect 3 intentional failures *)
+(* Expect 5 intentional failures *)
 module TestSet
 assume type elt
 assume logic val A : elt
@@ -28,3 +28,30 @@ val should_fail3: unit -> Tot unit
 let should_fail3 u =
   assert (mem C (union (singleton A) (singleton B)))
             
+
+module TestHeap
+open Set
+open Heap
+assume val x : ref int
+assume val y : ref int
+assume val h : heap
+assume DistinctXY: x <> y
+
+let test0 _ = assert (sel (upd h x 0) x = 0)
+let test1 _ = assert (sel (upd (upd h x 0) y 1) x = 0)
+let test2 _ = assert (sel (upd (upd h x 0) y 1) y = 0) //should fail
+let test3 _ = assert (sel (upd (upd h x 0) y 1) y = 1)
+let h1 = upd (upd h x 0) y 1
+let test5 _ = assert (equal h1 (upd (upd h y 1) x 0))
+let ys = Set.singleton (Ref y)
+let test6 _ = assert (equal h1 (concat h1 (restrict h1 (complement ys))))
+let test7 _ = assert (contains h1 x)
+let test8 _ = assert (contains h y ==> contains (upd h x 0) y)
+let test9 (x:ref int) =
+  assume (not (contains h x));
+  assert (equal (upd h x 0) (concat (upd h x 0) (restrict h (complement empty))))
+let test10 (x:ref int) (y:ref int) (h0:heap) (h1:heap) (h2:heap) =
+  admitP (h1 == concat h1 (restrict h0 (complement empty))) ();
+  admitP (h1 == upd h0 x 0) ();
+  admitP (~ (contains h1 y)) ();
+  assert false //should fail
